Dealt with Krivine

theories/CombinatoryLogic/Krivine.v
@@ -37,170 +37,14 @@ Inductive halt_cbn : list eterm -> list eterm -> term -> Prop :=
   | halt_lam ctx s :
       halt_cbn [] ctx (lam s).
 
-Lemma halt_cbnE ts ctx u : halt_cbn ts ctx u ->
-  match u with
-  | var 0 =>
-      match ctx with
-      | [] => False
-      | (closure ctx' t')::_ => halt_cbn ts ctx' t'
-      end
-  | var (S n) => 
-      match ctx with
-      | [] => False
-      | _::ctx' => halt_cbn ts ctx' (var n)
-      end
-  | app s t => halt_cbn ((closure ctx t) :: ts) ctx s
-  | lam s =>
-      match ts with
-      | [] => True
-      | t'::ts' => halt_cbn ts' (t'::ctx) s
-      end
-  end.
-Proof. by case. Qed.
-
-Fixpoint term_size (t : term) : nat :=
-  match t with
-  | var n => n
-  | app s t => 1 + term_size s + term_size t
-  | lam s => 1 + term_size s
-  end.
-
-Fixpoint eterm_size (u : eterm) : nat :=
-  let '(closure ctx t) := u in 1 + list_sum (map eterm_size ctx) + (term_size t).
-
-Definition context_size (ctx : list eterm) : nat :=
-  eterm_size (closure ctx (var 0)).
-
 Fixpoint eclosed (u : eterm) : Prop :=
   let '(closure ctx t) := u in bound (length ctx) t /\ Forall id (map eclosed ctx).
 
-(* example: elim /(measure_rect length) : l. *)
-Lemma measure_rect {X : Type} (f : X -> nat) (P : X -> Type) : 
-(forall x, (forall y, f y < f x -> P y) -> P x) -> forall (x : X), P x.
-Proof.
-  exact: (well_founded_induction_type (Wf_nat.well_founded_lt_compat X f _ (fun _ _ => id)) P).
-Qed.
-
-(* function composition *)
-Definition funcomp {X Y Z} (g : Y -> Z) (f : X -> Y) :=
-  fun x => g (f x).
-
-Arguments funcomp {X Y Z} (g f) /.
-
-(* stream cons *)
-Definition scons {X: Type} (x : X) (xi : nat -> X) :=
-  fun n => match n with | 0 => x | S n => xi n end.
-
-Fixpoint ren (xi : nat -> nat) (t : term) : term  :=
-  match t with
-  | var x => var (xi x)
-  | app s t => app (ren xi s) (ren xi t)
-  | lam t => lam (ren (scons 0 (funcomp S xi)) t)
-  end.
-
-Fixpoint subst (sigma: nat -> term)  (s: term) : term :=
-  match s with
-  | var n => sigma n
-  | app s t => app (subst sigma s) (subst sigma t)
-  | lam s => lam (subst (scons (var 0) (funcomp (ren S) sigma)) s)
-  end.
-
-Definition many_subst (ts : list term) (s : term) : term :=
-  subst (fun n => nth n ts (var (n - length ts))) s.
-
-Arguments many_subst ts !s /.
-
-(* recursively substitute each local context, rename all free varaibles to 0 *)
-Fixpoint flatten (u : eterm) : term :=
-  let '(closure ctx t) := u in ren (fun=> 0) (many_subst (map flatten ctx) t).
-
-
-Lemma flatten_var_0 t ctx :
-  flatten (closure (t :: ctx) (var 0)) = flatten t.
-Proof. move: t => [? ?]. by rewrite /= /many_subst /= ren_ren_term. Qed.
-
-Lemma flatten_var_S t ctx n :
-  flatten (closure (t :: ctx) (var (S n))) = flatten (closure ctx (var n)).
-Proof. done. Qed.
 
 Lemma Forall2_consE {X : Type} {P : X -> X -> Prop} {x1 l1 x2 l2} : 
   Forall2 P (x1::l1) (x2::l2) -> P x1 x2 /\ Forall2 P l1 l2.
 Proof. move=> H. by inversion H. Qed.
 
-Lemma many_subst_cons u ts s : ren (fun=> 0) (many_subst (u :: ts) s) = 
-  subst (funcomp (ren (fun=> 0)) (scons u var))
-    (if ren (fun=> 0) (many_subst ts (lam s)) is lam t then t else var 0).
-Proof.
-  rewrite /many_subst /= !ren_subst_term !subst_subst_term.
-  apply: ext_subst_term.
-  move=> [|n] /=; first done.
-  rewrite /funcomp /=. move: (nth _ _ _) => ?.
-  rewrite !subst_ren_term ren_as_subst_term.
-  apply: ext_subst_term. by case.
-Qed.
-
-(* halt_cbn is invariant closure flattening *)
-Lemma halt_cbn_flatten_iff {ts1 ts2 ctx1 ctx2 s1 s2} :
-  halt_cbn ts1 ctx1 s1 ->
-  map flatten ts1 = map flatten ts2 ->
-  flatten (closure ctx1 s1) = flatten (closure ctx2 s2) ->
-  halt_cbn ts2 ctx2 s2.
-Proof.
-  move=> H. elim: H ts2 ctx2 s2; clear ts1 ctx1 s1.
-  - move=> ts ctx t ctx' ? IH ts2 ctx2 s2.
-    rewrite flatten_var_0.
-    by move=> /IH /[apply].
-  - move=> ts1 ctx1 n t ? IH ts2 ctx2 s2.
-    rewrite flatten_var_S.
-    by move=> /IH /[apply].
-  - move=> ts1 ctx1 s t ? IH ts2 ctx2 s2.
-    elim /(measure_rect context_size): ctx2 s2.
-    move=> ctx2 IH' []. 
-    + (* s2 is (var n) *)
-      move: ctx2 IH' => [|[ctx'2 t'2] ctx2] IH'. { by case. }
-      move=> [|n].
-      * rewrite flatten_var_0.
-        move=> /= ??. apply: halt_var_0. apply: IH' => //=.
-        rewrite /context_size /=. lia.
-      * rewrite flatten_var_S.
-        move=> /= ??. apply: halt_var_S. apply: IH' => //=.
-        rewrite /context_size /=. lia.
-    + move=> ??? /= [] /IH {}IH ?.
-      apply: halt_app. apply: IH => //=.
-      by congr cons.
-    + done.
-  - move=> t1 ts1 ctx1 s1 ? IH [|t2 ts2] ctx2 s2; first done.
-    move=> [Ht1t2 ?].
-    elim /(measure_rect context_size): ctx2 s2.
-    move=> ctx2 IH' []. 
-    + (* s2 is (var n) *)
-      move: ctx2 IH' => [|[ctx'2 t'2] ctx2] IH'. { by case. }
-      move=> [|n].
-      * rewrite flatten_var_0.
-        move=> /= ?. apply: halt_var_0. apply: IH' => //=.
-        rewrite /context_size /=. lia.
-      * rewrite flatten_var_S.
-        move=> /= ?. apply: halt_var_S. apply: IH' => //=.
-        rewrite /context_size /=. lia.
-    + done.
-    + move=> s2 /= [Hs1s2]. apply: halt_lam_ts. apply: IH => //=.
-      by rewrite Ht1t2 !many_subst_cons /= Hs1s2.
-  - move=> ctx1 s1 [|t2 ts2] ctx2 s2; last done.
-    move=> _.
-    elim /(measure_rect context_size): ctx2 s2.
-    move=> ctx2 IH' []. 
-    + (* s2 is (var n) *)
-      move: ctx2 IH' => [|[ctx'2 t'2] ctx2] IH'. { by case. }
-      move=> [|n].
-      * rewrite flatten_var_0.
-        move=> /= ?. apply: halt_var_0. apply: IH' => //=.
-        rewrite /context_size /=. lia.
-      * rewrite flatten_var_S.
-        move=> /= ?. apply: halt_var_S. apply: IH' => //=.
-        rewrite /context_size /=. lia.
-    + done.
-    + move=> *. by apply: halt_lam.
-Qed.
 
 Lemma halt_cbn_ren_S {ts ctx u s} :
   halt_cbn ts ctx s ->
@@ -210,36 +54,6 @@ Proof.
   - by rewrite /= /many_subst !simpl_term.
 Qed.
 
-(* left-most outer-most call-by-name *)
-Inductive step : term -> term -> Prop :=
-  | stepLam s t    : step (app (lam s) t) (subst (scons t var) s)
-  | stepApp s s' t : step s s' -> step (app s t) (app s' t).
-
-Lemma stepE s t :
-  step s t ->
-  match s with
-  | app (lam s1) s2 => t = subst (scons s2 var) s1
-  | app (app s1 s2) s3 => exists s', t = app s' s3 /\ step (app s1 s2) s'
-  | _ => False
-  end.
-Proof.
-  elim; first done.
-  case; [done| |done].
-  move=> []; [done| |].
-  - move=> > ? [?] [-> ?].
-    eexists. split; [done|by apply: stepApp].
-  - move=> > ? ->. eexists. split; [done|by apply: stepLam].
-Qed.
-
-Lemma step_fun s t1 t2 : step s t1 -> step s t2 -> t1 = t2.
-Proof.
-  move=> H. elim: H t2.
-  - by move=> > /stepE ->.
-  - case.
-    + by move=> > /stepE.
-    + by move=> > ? IH t2 /stepE [?] [->] /IH ->.
-    + by move=> > /stepE.
-Qed.
 
 Fixpoint stepf (s : term) : option term :=
   match s with
@@ -371,35 +185,6 @@ Lemma many_subst_closed {ts t} : closed t -> many_subst ts t = t.
 Proof. move=> /subst_closed. by apply. Qed.
 
 
-
-Lemma step_halt_cbn s t ts ctx : closed s -> step s t ->
-  halt_cbn ts ctx s -> halt_cbn ts ctx t.
-Proof.
-  move=> Hs Hst. elim: Hst Hs ts ctx; clear s t.
-  - move=> s t /closed_app [Hs Ht] ts ctx /halt_cbnE /halt_cbnE.
-    move=> /halt_cbn_flatten_iff. apply; first done.
-    rewrite /= /many_subst /= !simpl_term. apply: ext_subst_term.
-    rewrite /funcomp /=. move=> [|n] /=; last done.
-    rewrite !simpl_term. apply: ext_subst_term.
-    move=> n. by rewrite /funcomp /= !simpl_term.
-  - move=> s s' t ? IH /closed_app [Hs Ht] ts ctx /halt_cbnE /IH {}IH.
-    apply: halt_app. by apply: IH.
-Qed.
-
-Lemma step_halt_cbn' s t ts ctx : closed s -> step s t ->
-  halt_cbn ts ctx t -> halt_cbn ts ctx s.
-Proof.
-  move=> Hs Hst. elim: Hst Hs ts ctx; clear s t.
-  - move=> s t /closed_app [Hs Ht] ts ctx H'.
-    apply: halt_app. apply: halt_lam_ts.
-    apply: (halt_cbn_flatten_iff H'); first done.
-    rewrite /= /many_subst /= !simpl_term. apply: ext_subst_term.
-    rewrite /funcomp /=. move=> [|n] /=; last done.
-    rewrite !simpl_term. apply: ext_subst_term.
-    move=> n. by rewrite /funcomp /= !simpl_term.
-  - move=> s s' t ? IH /closed_app [Hs Ht] ts ctx /halt_cbnE /IH {}IH.
-    apply: halt_app. by apply: IH.
-Qed.
 
 (* maybe this is needed? 
 Lemma halt_cbn_spec ts ctx s : halt_cbn ts ctx s ->
