theories/CombinatoryLogic/Plotkin2.v
@@ -240,9 +240,6 @@ Lemma t_trans' {A : Type} {R : relation A} {x x' y z : A} :
   x = x' -> clos_trans R x y -> clos_trans R y z -> clos_trans R x' z.
 Proof. move=> ->. by apply: t_trans. Qed.
 
-Lemma stepLam' s t t' : t' = (subst (scons t var) s) -> step (app (lam s) t) t'.
-Proof. move=> ->. by apply: stepLam. Qed.
-
 Lemma steps_to_colon s u : closed s -> clos_trans step (app (cbv_cbn s) u) (colon s u).
 Proof.
   elim: s u.
