theories/LambdaCalculus/Krivine_undec.v
@@ -1,0 +1,21 @@
+(* 
+  Undecidability Result(s):
+    Krivine machine halting (KrivineM_HALT)
+*)
+
+From Undecidability.Synthetic Require Import Undecidability.
+
+Require Import Undecidability.LambdaCalculus.Krivine.
+From Undecidability.LambdaCalculus.Reductions Require
+  wCBNclosed_to_KrivineM_HALT.
+
+Require Import Undecidability.LambdaCalculus.wCBN_undec.
+
+(* Undecidability of Krivine machine halting *)
+Theorem KrivineM_HALT_undec : undecidable KrivineM_HALT.
+Proof.
+  apply (undecidability_from_reducibility wCBNclosed_undec).
+  exact wCBNclosed_to_KrivineM_HALT.reduction.
+Qed.
+
+Check KrivineM_HALT_undec.
