theories/LambdaCalculus/Reductions/wCBNclosed_to_KM_HALT.v
@@ -1,6 +1,0 @@
-(*
-  Reduction from:
-    Weak call-by-name leftmost outermost normalization of closed terms (wCBNclosed)
-  to:
-    Krivine machine halting (KM_HALT)
-*)
